theories/Environment.v
@@ -1,0 +1,125 @@
+(** * Typing environments *)
+
+From MailboxTypes Require Export Types.
+From MailboxTypes Require Import Util.
+
+Require Import Lists.List.
+Import ListNotations.
+
+Generalizable All Variables.
+
+(** ** Definition of environments and operations on them *)
+Section environment_def.
+
+Context `{M : IMessage Message}.
+
+(** A type environment is represented as a list of option types.
+    For example the environment [[None, Some Int, Some Bool, None]]
+    represents
+    0 |-> None
+    1 |-> Int
+    2 |-> Bool
+    3 |-> None
+
+   This represented is chosen to keep avoid shifting de Bruijn indices
+   when splitting an environment.
+*)
+Definition Env := list (option TUsage).
+
+(** Lookup the type of an variable in an environment *)
+Fixpoint lookup (n : nat) (env : Env) : option TUsage :=
+  match n, env with
+  | _, nil => None
+  | 0, (None :: env') => None
+  | 0, (Some T :: env') => Some T
+  | S n', (_ :: env') => lookup n' env'
+  end.
+
+(** Definition 3.4 of environment subtyping.
+    Subtyping of environments includes weakening for unrestricted types.
+    This representation relates two environments of equal length, but
+    they may contain different amounts of types
+*)
+Inductive EnvironmentSubtype : Env -> Env -> Prop :=
+    EnvSubtypeEmpty : EnvironmentSubtype nil nil
+  | EnvSubtypeUn : forall env1 env2 T,
+      Unrestricted T ->
+      EnvironmentSubtype env1 env2 ->
+      EnvironmentSubtype (Some T :: env1) (None :: env2)
+  | EnvSubtypeSub : forall env1 env2 T1 T2,
+      Subtype T1 T2 ->
+      EnvironmentSubtype env1 env2 ->
+      EnvironmentSubtype (Some T1 :: env1) (Some T2 :: env2).
+
+(** Definition 3.8 of environment combination.
+    This representation relates three environments of equal length, but
+    they may contain different amounts of types
+*)
+Inductive EnvironmentCombination : Env -> Env -> Env -> Prop :=
+    EnvCombEmpty : EnvironmentCombination nil nil nil
+  | EnvCombLeft : forall env1 env2 env T,
+      EnvironmentCombination env1 env2 env ->
+      EnvironmentCombination (Some T :: env1) (None :: env2) (Some T :: env)
+  | EnvCombRight : forall env1 env2 env T,
+      EnvironmentCombination env1 env2 env ->
+      EnvironmentCombination (None :: env1) (Some T :: env2) (Some T :: env)
+  | EnvCombBoth : forall T env1 env2 env T1 T2,
+      EnvironmentCombination env1 env2 env ->
+      T1 ▷ T2 ~= T ->
+      EnvironmentCombination (Some T1 :: env1) (Some T2 :: env2) (Some T :: env).
+
+(** Definition 3.9 of disjoint environment combination.
+    This representation relates three environments of equal length, but
+    they may contain different amounts of types
+*)
+Inductive EnvironmentDisjointCombination : Env -> Env -> Env -> Prop :=
+    EnvDisCombEmpty : EnvironmentDisjointCombination nil nil nil
+  (* Special constructor for our representation of environments *)
+  (* TODO: Check if this is correct *)
+  | EnvDisCombNone : forall env1 env2 env,
+      EnvironmentDisjointCombination env1 env2 env ->
+      EnvironmentDisjointCombination (None :: env1) (None :: env2) (None :: env)
+  | EnvDisCombLeft : forall env1 env2 env T,
+      EnvironmentDisjointCombination env1 env2 env ->
+      EnvironmentDisjointCombination (Some T :: env1) (None :: env2) (Some T :: env)
+  | EnvDisCombRight : forall env1 env2 env T,
+      EnvironmentDisjointCombination env1 env2 env ->
+      EnvironmentDisjointCombination (None :: env1) (Some T :: env2) (Some T :: env)
+  | EnvDisCombBoth : forall env1 env2 env BT,
+      EnvironmentDisjointCombination env1 env2 env ->
+      EnvironmentDisjointCombination
+        (Some (TUBase BT) :: env1) (Some (TUBase BT) :: env2) (Some (TUBase BT) :: env).
+
+Inductive EnvironmentDisjointCombinationN : list Env -> Env -> Prop :=
+    EnvDisComb2 : forall env env1 env2,
+      EnvironmentDisjointCombination env1 env2 env ->
+      EnvironmentDisjointCombinationN [env1 ; env2] env
+  | EnvDisCombN : forall env env1 env2 env3 envList,
+      EnvironmentDisjointCombination env1 env2 env3 ->
+      EnvironmentDisjointCombinationN (env3 :: envList) env ->
+      EnvironmentDisjointCombinationN (env1 :: env2 :: envList) env.
+
+Definition returnEnvironment (env : Env) : Env := map_maybe returnUsage env.
+Definition secondEnvironment (env : Env) : Env := map_maybe secondUsage env.
+
+(** An environment is Base if it only contains base types *)
+Fixpoint BaseEnv (e : Env) : Prop :=
+  match e with
+  | nil => True
+  | (Some (TUBase _) :: env') => BaseEnv env'
+  | (None :: env') => BaseEnv env'
+  | _ => False
+  end.
+
+End environment_def.
+
+(** Notation for environments *)
+Declare Scope environment_scope.
+Open Scope environment_scope.
+
+Notation "Env1 ≤ₑ Env2" := (EnvironmentSubtype Env1 Env2) (at level 80) : environment_scope.
+Notation "Env1 ▷ₑ Env2 ~= Env" := (EnvironmentCombination Env1 Env2 Env) (at level 80) : environment_scope.
+Notation "Env1 +ₑ Env2 ~= Env" := (EnvironmentDisjointCombination Env1 Env2 Env) (at level 80) : environment_scope.
+Notation "[ Env1 ]+ₑ ~= Env" := (EnvironmentDisjointCombinationN Env1 Env) (at level 80) : environment_scope.
+Notation "⌊ Env ⌋ₑ" := (returnEnvironment Env) : environment_scope.
+Notation "⌈ Env ⌉ₑ" := (secondEnvironment Env) : environment_scope.
